<?xml version="1.0" encoding="UTF-8"?>
<rdf:RDF xml:base="http://dd.eionet.europa.eu/schema.rdf"
	xmlns:rdf="http://www.w3.org/1999/02/22-rdf-syntax-ns#"
	xmlns:dct="http://purl.org/dc/terms/"
	xmlns:owl="http://www.w3.org/2002/07/owl#"
	xmlns:rdfs="http://www.w3.org/2000/01/rdf-schema#">

	<owl:Ontology rdf:about="">
		<rdfs:label>Data dictionary schema</rdfs:label>
		<owl:versionInfo>$Id$</owl:versionInfo>
		<dct:creator rdf:resource="http://www.eionet.europa.eu/users/roug"/>
		<dct:contributor rdf:resource="http://www.eionet.europa.eu/users/heinlja"/>
	</owl:Ontology>

	<!-- Classes -->

	<rdfs:Class rdf:ID="TableSchema">
		<rdfs:label>Table schema</rdfs:label>
		<rdfs:comment>A table schema is an RDF document that contains the RDF schema for a table</rdfs:comment>
		<rdfs:subClassOf rdf:resource="http://www.w3.org/2002/07/owl#Ontology"/>
	</rdfs:Class>

	<rdfs:Class rdf:ID="DatasetSchema">
		<rdfs:label>Dataset schema</rdfs:label>
		<rdfs:comment>A dataset schema is an RDF document that contains the RDF schema for a dataset</rdfs:comment>
		<rdfs:subClassOf rdf:resource="http://www.w3.org/2002/07/owl#Ontology"/>
	</rdfs:Class>

	<rdfs:Class rdf:ID="SchemaSet">
		<rdfs:label>Set of XML schemas</rdfs:label>
		<rdfs:comment>A schema set is a grouping of XML schemas that depend on each other in some way.</rdfs:comment>
	</rdfs:Class>

	<rdfs:Class rdf:ID="SiteCode">
        <rdfs:label>Site code</rdfs:label>
        <rdfs:comment>Site code is a unique numeric identifier of site records in the Common Database of Designated Areas which is annually updated in one of the EEA's priority dataflows.</rdfs:comment>
    </rdfs:Class>

	<!-- Properties -->

	<rdf:Property rdf:ID="hasSchema">
		<rdfs:label>Has schema</rdfs:label>
		<rdfs:comment>Link from a schema set to a schema member.</rdfs:comment>
		<rdfs:domain rdf:resource="#SchemaSet"/>
		<rdfs:range rdf:resource="http://cr.eionet.europa.eu/ontologies/contreg.rdf#XMLSchema"/>
	</rdf:Property>

	<rdf:Property rdf:ID="usesVocabulary">
		<rdfs:label>Uses vocabulary</rdfs:label>
		<rdfs:comment>The property value must be a literal listed as the skos:prefLabel in a member of the skos:Collection referenced.</rdfs:comment>
		<rdfs:range rdf:resource="http://www.w3.org/2004/02/skos/core#Collection"/>
	</rdf:Property>

	<rdf:Property rdf:ID="siteCode">
        <rdfs:label>Site code</rdfs:label>
        <rdfs:comment>Site code is a unique numeric identifier of site records in the Common Database of Designated Areas which is annually updated in one of the EEA's priority dataflows.</rdfs:comment>
        <rdfs:domain rdf:resource="#SiteCode"/>
        <rdfs:range rdf:resource="http://www.w3.org/2001/XMLSchema#int"/>
    </rdf:Property>

    <rdf:Property rdf:ID="siteName">
        <rdfs:label>Site name</rdfs:label>
        <rdfs:comment>Name of a site that has a site code assigned to it.</rdfs:comment>
        <rdfs:domain rdf:resource="#SiteCode"/>
        <rdfs:range rdf:resource="http://www.w3.org/2001/XMLSchema#string"/>
    </rdf:Property>

    <rdf:Property rdf:ID="status">
        <rdfs:label>Site code status</rdfs:label>
        <rdfs:comment>A site code's status. One of AVAILABLE, ALLOCATED, ASSIGNED, DISAPPEARED, DELETED.</rdfs:comment>
        <rdfs:domain rdf:resource="#SiteCode"/>
        <rdfs:range rdf:resource="http://www.w3.org/2001/XMLSchema#string"/>
    </rdf:Property>

    <rdf:Property rdf:ID="countryAllocated">
        <rdfs:label>Site code country</rdfs:label>
        <rdfs:comment>Country to which a site is allocated.</rdfs:comment>
        <rdfs:domain rdf:resource="#SiteCode"/>
        <rdfs:range rdf:resource="http://rdfdata.eionet.europa.eu/eea/ontology/Country"/>
    </rdf:Property>

    <rdf:Property rdf:ID="yearCreated">
        <rdfs:label>Site code creation year</rdfs:label>
        <rdfs:comment>Year when a site code was created.</rdfs:comment>
        <rdfs:domain rdf:resource="#SiteCode"/>
        <rdfs:range rdf:resource="http://www.w3.org/2001/XMLSchema#gYear"/>
    </rdf:Property>
    
    <rdf:Property rdf:ID="hasTable">
		<rdfs:label>Has table</rdfs:label>
		<rdfs:comment>Link from a dataset to its belonging table</rdfs:comment>
	</rdf:Property>

</rdf:RDF>
